src/ErrorStringConstants.v
@@ -13,3 +13,11 @@ Definition errStr_app_auth_tok : StringT. Admitted.
 Definition errStr_dispatch_error : StringT. Admitted.
 
 Definition errStr_cvm_error : StringT. Admitted.
+
+Definition errStr_decryption_prim : StringT. Admitted.
+
+Definition errStr_et_size : StringT. Admitted.
+
+Definition errStr_lib_supports_man_check : StringT. Admitted.
+
+Definition errStr_lib_supports_man_app_check : StringT. Admitted.
